haskell/adi/Macro.hs
@@ -1,0 +1,23 @@
+module  Macro
+    (   eSum
+    ,   eFac
+    )   where
+
+import Op
+import Syntax
+
+-- \x y -> x + y
+eSum :: String -> String -> Expr
+eSum x y = 
+    (eLam x
+        (eLam y
+            (eOp add (eVar x) (eVar y))))
+
+eFac :: String -> String -> Expr
+eFac f n =
+    (eRec f
+       (eLam n
+            (eIf (eVar n) (eNum 1) 
+                (eOp mul (eVar n) 
+                    (eApp (eVar f) 
+                        (eOp add (eVar n) (eNum (-1)))))))) 
