haskell/adi/Test/Debug.hs
@@ -1,0 +1,21 @@
+module  Test.Debug
+    (   main
+    ,   e1, e2, e3
+    )   where
+
+import Macro
+import Syntax
+import Interpret
+
+main :: IO ()
+main = do
+   evalIO e3
+
+e1 :: Expr
+e1 = eLam "x" (eVar "x") 
+
+e2 :: Expr
+e2 = eApp (eLam "x" (eLam "y" (eVar "x"))) (eNum 4)
+
+e3 :: Expr 
+e3 = eApp (eFac "f" "n") (eNum 5)
