haskell/aop/Steep.hs
@@ -1,3 +1,5 @@
+{-# LANGUAGE LambdaCase             #-}
+
 module Steep
     (   main
     ,   steep1
@@ -5,22 +7,45 @@ module Steep
 
 import Test.Hspec
 import Test.QuickCheck
---import Data.Functor.Foldable
+import Data.Functor.Foldable
 
 main :: IO ()
 main = hspec $ describe "Testing equivalence of implementations" $ do
     spec1
+    spec2
+    spec3
 
 spec1 :: Spec
-spec1 = it "Checked steep1 ~ steep1" $ do
+spec1 = it "Checked steep1 ~ steep2" $ do
     property prop1 
 
+spec2 :: Spec
+spec2 = it "Checked fst . steep2_ == sum" $ do
+    property prop2 
+
+spec3 :: Spec
+spec3 = it "Checked steep2 (x : xs) == x > sum xs && steep2 xs" $ do
+    property prop3 
+
 prop1 :: [Int] -> Bool
-prop1 xs = steep1 xs == steep1 xs
+prop1 xs = steep1 xs == steep2 xs
+
+prop2 :: [Int] -> Bool
+prop2 xs = (fst . steep2_) xs == sum xs
+
+prop3 :: Int -> [Int] -> Bool
+prop3 x xs = steep2 (x : xs) == (x > sum xs && steep2 xs)
 
 -- Quadratic complexity. Need to find implementation with linear complexity.
 steep1 :: (Num a, Ord a) => [a] -> Bool
 steep1 [] = True
 steep1 (x : xs) = x > sum xs && steep1 xs
 
+steep2_ :: (Num a, Ord a) => [a] -> (a,Bool)
+steep2_ = cata $ \case
+    Nil             -> (0,True)
+    Cons x (s,b)    -> (s + x, x > s && b)
+
+steep2 :: (Num a, Ord a) => [a] -> Bool
+steep2 = snd . steep2_
 
