coq/set/Core/Replacement.v
@@ -4,9 +4,15 @@ Require Import Utils.LEM.
 Require Import Utils.Filter.
 
 Require Import Core.Set.
+Require Import Core.Incl.
 Require Import Core.Elem.
-Require Import Core.Compatible.
+Require Import Core.Equal.
+Require Import Core.ToList.
 Require Import Core.Functional.
+Require Import Core.Compatible.
+Require Import Core.Extensionality.
+
+Require Import Normal.Normal.
 
 (* Axiom schema of replacement assuming LEM for our Coq meta-logic.             *)
 Theorem replacememtLEM : forall (p:set -> set -> Prop),
@@ -17,8 +23,27 @@ Theorem replacememtLEM : forall (p:set -> set -> Prop),
         exists (y:set), forall (z:set),
             z :: y <-> exists (u:set), u :: x /\ p u z.
 Proof.
-   intros p L C F x. 
-   remember (fun (z:set) => exists (u:set), u :: x /\ p u z) as q eqn:Eq. 
-   remember (toList x) as xs eqn:Ex.
-
+    intros p L C F x. 
+    remember (toList x) as xs eqn:H1.
+    remember (fun x y => p x y /\ Normal y) as q eqn:Q.
+    assert (forall (x:set) (y y':set), q x y -> q x y' -> y = y') as H2.
+    { rewrite Q. intros u y y' [H3 H4] [H5 H6]. apply normalEqualSame.
+        { assumption. }
+        { assumption. }
+        { apply (F u); assumption. } }
+    assert (exists (ys:list set), forall (y:set), 
+        In y ys <-> exists (u:set), In u xs /\ q u y) as H3.
+    { apply filterReplace; assumption. }
+    destruct H3 as [ys H3]. exists (fromList ys). intros z. split; intros H4.
+    - rewrite toListElem, toListFromList in H4. destruct H4 as [z' [H4 [H5 H6]]].
+      apply H3 in H4. rewrite Q in H4. destruct H4 as [u [H7 [H8 H9]]].    
+      exists u. split.
+        + apply toListElem. exists u. split.
+            { rewrite <- H1. assumption. }
+            { split; apply inclRefl. }
+        + apply (C u u z' z).
+            { apply equalRefl. }
+            { apply doubleIncl. split; assumption. }
+            { assumption. }
+    -
 Show.
